# Ontologisches Beweis

- author: lbolla
- category: nice-words
- tags: 
- summary: 
- date: 2006-08-11 21:50:05

----------------

    Ass.1: P(φ).P(ψ) ⊃ P(φ.ψ)
    Ass.2: P(φ) ∨ P(-φ)

    Def.1: G(x) ≡ (φ)[P(φ) ⊃ φ(x)]
    Def.2: φ Ess. x ≡ (ψ)[ψ(x) ⊃ N(y){φ(y) ⊃ ψ(y)]]

    Ass.3a: P(φ) ⊃ NP(φ)
    Ass.3b: ∼P(φ) ⊃ N∼P(φ)

    Theo.1: G(x) ⊃ G Ess. x

    Def.3: E(x) ≡ (φ)[φ Ess. x ⊃ N(∃x) φ(x)]

    Ass.4: P(E)

    Theo.2: G(x) ⊃ N(∃y)G(y)

    Therefore:
    (∃x)G(x) ⊃ N(∃y)G(y)
    M(∃x)G(x) ⊃ MN(∃y)G(y)
    M(∃x)G(x) ⊃ N(∃y)G(y)

    Ass.5: P(φ).N(φ⊃ψ):⊃P(ψ) 

K. Gödel, 1970
